Symbolic simulation and fixed a bug in code

arm/proofs/aes_decrypt.ml
@@ -4,31 +4,33 @@
  *)
 
 use_file_raise_failure := true;;
+arm_print_log := true;;
 
 needs "arm/proofs/base.ml";;
+loadt "arm/proofs/aes_decrypt_spec.ml";;
 
 print_literal_from_elf "arm/aes-xts/aes256_decrypt.o";;
 
-let aes256_decrypt_mc = define_assert_from_elf "aes256_decrypt" "arm/aes-xts/aes256_decrypt.o"
+let aes256_decrypt_mc = define_assert_from_elf "aes256_decrypt_mc" "arm/aes-xts/aes256_decrypt.o"
 [
-  0xb940f046;       (* arm_LDR W6 X2 (Immediate_Offset (word 240)) *)
-  0x4cdf7040;       (* arm_LDR Q0 X2 (Postimmediate_Offset (word 16)) *)
+  0xb940f046;       (* arm_LDR W6 X2 (Immediate_Offset (word 0xf0)) *)
+  0x4cdf7040;       (* arm_LDR Q0 X2 (Postimmediate_Offset (word 0x10)) *)
   0x4c407026;       (* arm_LDR Q6 X1 No_Offset *)
-  0x510008c6;       (* arm_SUB W6 W6 (rvalue (word 2)) *)
-  0x4cdf7041;       (* arm_LDR Q1 X2 (Postimmediate_Offset (word 16)) *)
+  0x510008c6;       (* arm_SUB W6 W6 (rvalue (word 0x2)) *)
+  0x4cdf7041;       (* arm_LDR Q1 X2 (Postimmediate_Offset (word 0x10)) *)
   0x4e285806;       (* arm_AESD Q6 Q0 *)
   0x4e2878c6;       (* arm_AESIMC Q6 Q6 *)
-  0x4cdf7840;       (* arm_LDR Q0 X2 (Postimmediate_Offset (word 16)) *)
-  0x710008c6;       (* arm_SUBS W6 W6 (rvalue (word 2)) *)
+  0x4cdf7840;       (* arm_LDR Q0 X2 (Postimmediate_Offset (word 0x10)) *)
+  0x710008c6;       (* arm_SUBS W6 W6 (rvalue (word 0x2)) *)
   0x4e285826;       (* arm_AESD Q6 Q1 *)
   0x4e2878c6;       (* arm_AESIMC Q6 Q6 *)
-  0x4cdf7841;       (* arm_LDR Q1 X2 (Postimmediate_Offset (word 16)) *)
-  0x54ffff2c;       (* arm_BGT (word 2097124) *)
+  0x4cdf7841;       (* arm_LDR Q1 X2 (Postimmediate_Offset (word 0x10)) *)
+  0x54ffff2c;       (* arm_BGT (word 0x1fffe4) *)
   0x4e285806;       (* arm_AESD Q6 Q0 *)
   0x4e2878c6;       (* arm_AESIMC Q6 Q6 *)
-  0x4c407880;       (* arm_LDR Q0 X4 No_Offset *)
+  0x4c407840;       (* arm_LDR Q0 X2 No_Offset *)
   0x4e285826;       (* arm_AESD Q6 Q1 *)
-  0x6e201cc6;       (* arm_EOR_VEC Q6 Q6 Q0 128 *)
+  0x6e201cc6;       (* arm_EOR_VEC Q6 Q6 Q0 0x80 *)
   0x4c007806        (* arm_STR Q6 X0 No_Offset *)
 ];;
 
@@ -36,36 +38,47 @@ let AES256_DECRYPT_EXEC = ARM_MK_EXEC_RULE aes256_decrypt_mc;;
 
 (* TODO: Could this be better? read(memory :> bytes(key, 240) = all_k) *)
 let AES256_DECRYPT_CORRECT = prove(
-  `!out in key ib k0 k1 k2 k3 k4 k5 k6 k7 k8 k9 k10 k11 k12 k13 k14 pc.
-    nonoverlapping (word pc,LENGTH aes256_decrypt_mc) (out,16)
+  `!plaintext ciphertext key ib k0 k1 k2 k3 k4 k5 k6 k7 k8 k9 k10 k11 k12 k13 k14 pc.
+    nonoverlapping (word pc,LENGTH aes256_decrypt_mc) (plaintext,16)
     ==> ensures arm
       // precondition
-      (\s. aligned_bytes_loaded s (word pc) aes256_encrypt_mc /\
+      (\s. aligned_bytes_loaded s (word pc) aes256_decrypt_mc /\
            read PC s = word pc /\
-           C_ARGUMENTS [out; in; key] s /\
-           read(memory :> bytes(in, 16)) s = ib /\
-           read(memory :> bytes(word_add key (word 240), 4)) = word 13 /\
-           read(memory :> bytes(key, 16)) = k0 /\
-           read(memory :> bytes((word_add key (word 16)), 16)) = k1 /\
-           read(memory :> bytes((word_add key (word 32)), 16)) = k2 /\
-           read(memory :> bytes((word_add key (word 48)), 16)) = k3 /\
-           read(memory :> bytes((word_add key (word 64)), 16)) = k4 /\
-           read(memory :> bytes((word_add key (word 80)), 16)) = k5 /\
-           read(memory :> bytes((word_add key (word 96)), 16)) = k6 /\
-           read(memory :> bytes((word_add key (word 112)), 16)) = k7 /\
-           read(memory :> bytes((word_add key (word 128)), 16)) = k8 /\
-           read(memory :> bytes((word_add key (word 144)), 16)) = k9 /\
-           read(memory :> bytes((word_add key (word 160)), 16)) = k10 /\
-           read(memory :> bytes((word_add key (word 176)), 16)) = k11 /\
-           read(memory :> bytes((word_add key (word 192)), 16)) = k12 /\
-           read(memory :> bytes((word_add key (word 208)), 16)) = k13 /\
-           read(memory :> bytes((word_add key (word 224)), 16)) = k14)
+           C_ARGUMENTS [plaintext; ciphertext; key] s /\
+           read(memory :> bytes128 ciphertext) s = ib /\
+           read(memory :> bytes32 (word_add key (word 240))) s = word 14 /\
+           read(memory :> bytes128 key) s = k0 /\
+           read(memory :> bytes128 (word_add key (word 16))) s = k1 /\
+           read(memory :> bytes128 (word_add key (word 32))) s = k2 /\
+           read(memory :> bytes128 (word_add key (word 48))) s = k3 /\
+           read(memory :> bytes128 (word_add key (word 64))) s = k4 /\
+           read(memory :> bytes128 (word_add key (word 80))) s = k5 /\
+           read(memory :> bytes128 (word_add key (word 96))) s = k6 /\
+           read(memory :> bytes128 (word_add key (word 112))) s = k7 /\
+           read(memory :> bytes128 (word_add key (word 128))) s = k8 /\
+           read(memory :> bytes128 (word_add key (word 144))) s = k9 /\
+           read(memory :> bytes128 (word_add key (word 160))) s = k10 /\
+           read(memory :> bytes128 (word_add key (word 176))) s = k11 /\
+           read(memory :> bytes128 (word_add key (word 192))) s = k12 /\
+           read(memory :> bytes128 (word_add key (word 208))) s = k13 /\
+           read(memory :> bytes128 (word_add key (word 224))) s = k14)
       // postcondition
-      // TODO: Nevine will figure out the post condition for output
-      // hint: use the aes256_encrypt from aes_encrypt_spec
-      (\s. read PC s = word (pc + LENGTH aes256_encrypt_mc) /\
-           )
+      (\s. read PC s = word (pc + LENGTH aes256_decrypt_mc) /\
+           read (memory :> bytes128 plaintext) s = 
+             aes256_decrypt ib [k0; k1; k2; k3; k4; k5; k6; k7; k8; k9; k10; k11; k12; k13; k14]
+        )
       // MAYCHANGE
-      ()`,
+      (MAYCHANGE [PC])`,
+  MAP_EVERY X_GEN_TAC
+   [`plaintext:int64`; `ciphertext:int64`; `key:int64`; 
+    `ib:int128`; `k0:int128`; `k1:int128`; `k2:int128`; 
+    `k3:int128`; `k4:int128`; `k5:int128`; `k6:int128`; 
+    `k7:int128`; `k8:int128`; `k9:int128`; `k10:int128`; 
+    `k11:int128`; `k12:int128`; `k13:int128`; `k14:int128`; `pc:num`] THEN
+  REWRITE_TAC[C_ARGUMENTS; SOME_FLAGS;NONOVERLAPPING_CLAUSES] THEN
+  REWRITE_TAC [(REWRITE_CONV [aes256_decrypt_mc] THENC LENGTH_CONV) `LENGTH aes256_decrypt_mc`] THEN
+  DISCH_THEN(REPEAT_TCL CONJUNCTS_THEN ASSUME_TAC) THEN
+  ENSURES_INIT_TAC "s0" THEN
+  ARM_ACCSTEPS_TAC AES256_DECRYPT_EXEC [] (1--59) THEN
   CHEAT_TAC
-)
+);;
